First pass at insert front

proofs/Vector.v
@@ -4,6 +4,7 @@ Require Import Nat.
 Require Import List.
 Import ListNotations.
 From Coq Require Import Omega.
+From Coq Require Import Logic.FunctionalExtensionality.
 
 From RRB Require Import Prelude.
 
@@ -23,16 +24,22 @@ Definition size := nat.
 (* The main datatype. *)
 Inductive tree {A : Set} : Set :=
 | Leaf : list size -> list A -> tree
-| Node : height    -> list size -> list tree -> tree.
+| Node : height -> list size -> list tree -> tree.
 
 (* The type exported out of this module *)
 Definition vector {A : Set} := tree (A := A).
 
 (* Well this is technically not correct (Leaf doesn't have sizes), but OK for now. *)
-Definition sizes {A : Set} (tr : @vector A) : list nat :=
+Definition get_sizes {A : Set} (tr : @vector A) : list nat :=
   match tr with
   | Leaf szs _   => szs
   | Node _ szs _ => szs
+  end.
+
+Definition get_height {A : Set} (tr : @vector A) : nat :=
+  match tr with
+  | Leaf _ _    => 0
+  | Node ht _ _ => ht
   end.
 
 (* ---------------------------------- *)
@@ -49,20 +56,34 @@ Definition vec_length {A : Set} (tr : @vector A) : nat :=
   end.
 
 Lemma vec_length_sizes {A : Set} :
-  forall (tr : vector),  (vec_length tr > 0) -> (@sizes A tr) <> [].
+  forall (tr : vector),  (vec_length tr > 0) -> (@get_sizes A tr) <> [].
 Proof.
   intros. induction tr.
-  + unfold vec_length in H. unfold sizes.
+  + unfold vec_length in H. unfold get_sizes.
     apply length_gt_zero_iff_not_nil. apply H.
-  + unfold sizes. unfold vec_length in H.
+  + unfold get_sizes. unfold vec_length in H.
     induction l.
     - apply zero_gt_zero_false in H. unfold not. intro. apply H.
     - apply cons_not_empty.
 Qed.
 
+(* Should these things be written down as specs instead ? *)
+
 Axiom leaf_sizes_elems :
   forall {A : Set} (szs : list size) (ns : list A) (tr : @vector A),
-    tr = Leaf szs ns -> length szs = length ns.
+  tr = Leaf szs ns -> length szs = length ns.
+
+Axiom leaf_sizes_elems_m :
+  forall {A : Set} (szs : list size) (ns : list A) (tr : @vector A),
+  tr = Leaf szs ns -> length ns <= m.
+
+Axiom node_sizes_elems : forall {A : Set}
+  (ht : nat) (szs : list size) (trs : list (@vector A)) (tr : @vector A),
+   tr = Node ht szs trs -> length szs = length trs.
+
+Axiom node_sizes_elems_m : forall {A : Set}
+  (ht : nat) (szs : list size) (trs : list (@vector A)) (tr : @vector A),
+  tr = Node ht szs trs -> length trs <= m.
 
 Lemma vec_length_leaves_sizes {A : Set} :
   forall (tr : vector) (szs : list size) (ns : list A),
@@ -79,14 +100,25 @@ Qed.
 
 (* Not using bit operations for now *)
 Definition index_of (ht : height) (i : nat) : nat :=
-  (i / (pow m ht)) mod m.
+  (i / (m ^ ht)) mod m.
+
+Lemma index_of_lt_m {A : Set} : forall (ht i : nat), m > 0 -> index_of ht i < m.
+Proof.
+  intros. unfold index_of. unfold modulo. destruct m.
+  + apply H.
+  + omega.
+Qed.
+
+Axiom nooo : forall {A : Set}
+  (ht : nat) (szs : list size) (trs : list (@vector A)) (tr : @vector A) (idx : nat),
+  (tr = Node ht szs trs) -> (idx < vec_length tr) -> index_of ht idx < length szs.
 
 Fixpoint check_slot_default
   (sz_js : list (nat * nat)) (idx : nat) (default : nat) : nat :=
   match sz_js with
   | [] => default
-  | (sz , j) :: rst => if leb sz idx
-                       then check_slot_default rst idx default
+  | (sz , j) :: rst => if sz <? idx
+                       then check_slot_default rst idx j
                        else j
   end.
 
@@ -94,12 +126,9 @@ Definition check_slot' :
   forall (sz_js : list (nat * nat)) (idx : nat), sz_js <> [] -> nat.
   refine (fix f (sz_js : list (nat * nat)) (idx : nat) :=
               match sz_js with
-              | []              => fun pf  => _
+              | [] => fun pf  => _
               | (sz , j) :: rst =>
-                  fun _ =>
-                    if leb sz idx
-                    then check_slot_default rst idx j
-                    else j
+                  fun _ => check_slot_default rst idx j
               end).
     congruence.
 Defined.
@@ -108,18 +137,35 @@ Definition check_slot
   (s : { sz_js : list (nat * nat) | sz_js <> [] }) (idx : nat) : nat :=
   check_slot' (proj1_sig s) idx (proj2_sig s).
 
-Definition indexInNode
-  (ht : height) (szs : list size) (idx : nat) : (nat * nat) :=
-  let slot     := index_of ht idx in
-  let sz_js    := skipn slot (combine szs (seq 0 (length szs))) in
-  let slot'    := match sz_js with
-                  | []      => slot
-                  | a :: b  => check_slot (exist _ (a :: b) (cons_not_empty a b)) idx
-                  end
-  in let idx' := idx - (if eqb slot' 0
-                        then 0
-                        else nth (slot' - 1) szs 0)
-     in (slot' , idx').
+(*
+
+Want to prove:
+
+    (1) slot = index_of ht idx and slot < length szs
+
+    (2) slot' = check_slot sz_js idx and slot' < length szs
+
+We know:
+
+    (1) forall tr = Node ht szs trs, length szs = length trs.
+
+*)
+
+Definition indexInNode : forall {A : Set}
+  (tr : vector) (ht : height) (szs : list size) (idx : nat),
+  idx < (@vec_length A tr) -> (nat * nat).
+  refine (fun A tr ht szs idx idx_lt_vec_len =>
+            let slot  := index_of ht idx in
+            let sz_js := skipn slot (combine szs (seq 0 (length szs))) in
+            match sz_js with
+            | [] => _
+            | a :: b => let slot' := check_slot (exist _ (a :: b) (cons_not_empty a b)) idx in
+                        let idx' := idx - (if eqb slot' 0
+                                           then 0
+                                           else strong_nth szs (slot' - 1) _)
+                        in (slot' , idx')
+            end).
+  Admitted.
 
 Definition get {A : Set}
    (tr : vector) (s : { idx : nat | (idx < @vec_length A tr) }) (default : A) : A.
@@ -135,8 +181,102 @@ Definition get {A : Set}
     - apply tr.
 Defined.
 
-(* Compute (1 - 1). *)
-(* Definition test1 := [ 4 ; 6; 8; 16 ]. *)
-(* Compute (skipn 2 test1). *)
-(* Compute (seq 0 (length test1)). *)
-(* Compute (indexInNode 1 test1 10). *)
+(* ---------------------------------- *)
+(* -- Insert front/back               *)
+(* ---------------------------------- *)
+
+Inductive wherE : Set := Front | Back.
+
+Fixpoint mkLeafAtHeight {A : Set} (ht : height) (v1 : A) : (vector) :=
+  match ht with
+  | O => Leaf [1] [v1]
+  | S n => Node ht [1] [mkLeafAtHeight n v1]
+  end.
+
+Definition join {A : Set} (a : @vector A) (b : @vector A) : (@vector A) :=
+  Node (get_height a + 1) [ vec_length a ; (vec_length a + vec_length b) ] [a ; b].
+
+Lemma length_not_empty_inv {A B : Set} :
+  forall (xs : list A) (ys : list B),
+  length xs = length ys -> xs <> [] -> ys <> [].
+Proof. Admitted.
+
+
+Definition tryBottom : forall {A : Set}
+  (whr : wherE) (tr : @vector A) (v1 : A), option (@vector A).
+  refine
+    (fix f {A : Set} (whr : wherE) (tr : @vector A) (v1 : A) : option (@vector A) :=
+       ((match tr as tr' return tr = tr' -> option (vector) with
+         | Leaf szs ns =>
+           if length ns <? m
+           then match whr with
+                | Front => fun _ => Some (Leaf (1 :: szs) (v1 :: ns))
+                | Back  => fun _ => Some (Leaf (szs ++ [1]) (ns ++ [v1]))
+                end
+           else fun _ => None
+         | Node ht szs trs =>
+           fun pf_tr =>
+             (match trs as trs' return trs = trs' -> option (vector) with
+              | [] => fun _ => Some (Node ht [1] [mkLeafAtHeight (ht - 1) v1])
+              | hd :: rst  =>
+                fun pf_trs' =>
+                  let node_to_try := match whr with
+                                     | Front => strong_head trs _
+                                     | Back  => strong_last trs _
+                                     end in
+                  (* If we recur on node_to_try, it upsets Coq's termination checker *)
+                  match (f whr hd v1) with
+                  | Some has_v =>
+                    match whr with
+                    | Front => let hd_szs := strong_head szs _ in
+                               let tl_szs := tl szs in
+                               let szs'   := (1 + hd_szs) :: tl_szs in
+                               let trs'   := has_v :: tl trs in
+                               Some (Node ht szs' trs')
+                    | Back  => let last_szs := strong_last szs _ in
+                               let szs'     := removelast szs ++ [1 + last_szs] in
+                               let trs'     := removelast trs ++ [has_v] in
+                               Some (Node ht szs' trs')
+                    end
+                  | None =>
+                    if length trs <? m
+                    then let branch := mkLeafAtHeight (ht - 1) v1 in
+                         let szs'   := (match whr with
+                                        | Front => 1 :: (map (fun x => x + 1) szs)
+                                        | Back  => let last_szs := strong_last szs _ in
+                                                   szs ++ [1 + last_szs]
+                                        end) in
+                         let trs'   := (match whr with
+                                        | Front => branch :: trs
+                                        | Back  => trs ++ [branch]
+                                        end) in
+                         Some (Node ht szs' trs')
+                    else None
+                  end
+              end) (eq_refl trs)
+         end) (eq_refl tr))).
+  Unshelve.
+  (* when tryBottom succeeds, szs <> [] *)
+  + apply length_not_empty_inv with (hd :: rst).
+    rewrite node_sizes_elems with ht szs (hd :: rst) tr. auto.
+    rewrite <- pf_trs'. apply pf_tr. apply (cons_not_empty hd rst).
+  + apply length_not_empty_inv with (hd :: rst).
+    rewrite node_sizes_elems with ht szs (hd :: rst) tr. auto.
+    rewrite <- pf_trs'. apply pf_tr. apply (cons_not_empty hd rst).
+  + apply length_not_empty_inv with (hd :: rst).
+    rewrite node_sizes_elems with ht szs (hd :: rst) tr. auto.
+    rewrite <- pf_trs'. apply pf_tr. apply (cons_not_empty hd rst).
+  (* node_to_try => trs <> [] *)
+  + rewrite pf_trs'. apply (cons_not_empty hd rst).
+  + rewrite pf_trs'. apply (cons_not_empty hd rst).
+Qed.
+
+Definition insert {A : Set} (whr : wherE) (tr : vector) (v : A) : vector :=
+  match tryBottom whr tr v with
+  | Some has_v => has_v
+  | None => match whr with
+            | Front => join (mkLeafAtHeight (get_height tr) v) tr
+            | Back  => join tr (mkLeafAtHeight (get_height tr) v)
+            end
+
+  end.
